Attempt at new bind framing

ulib/experimental/SteelT.FramingBind.fst
@@ -17,31 +17,59 @@ let returnc (a:Type u#a) (x:a) (#[@resolve_framing] p:a -> hprop)
 
 open Steel.Memory.Tactics
 
-let can_be_split_into_forall (#a:Type) (outer inner:post_t a) (delta:pre_t)
-  = forall (x:a). can_be_split_into (outer x) (inner x) delta
+let can_be_split_into_forall (#a:Type) (outer inner delta:post_t a)
+  = forall (x:a). can_be_split_into (outer x) (inner x) (delta x)
 
+let can_be_split_into_forall_2 (#a #b:Type)
+  (outer:post_t b) (inner:a -> post_t b) (delta:post_t a)
+  = forall (x:a) (y:b). can_be_split_into (outer y) (inner x y) (delta x)
+
+(*
+outer_pre <==>
+pre_f * frame_f               // emp * emp
+
+x := f ()
+
+post_f x * frame_f            // ref x * emp
+
+<==>
+
+pre_g x * frame_g x           // emp * ref x
+
+y := g x ()
+
+post_g x y * frame_g x        // ref y * ref x
+
+<==> outer_post y
+*)
 let bind (a:Type) (b:Type)
   (#[@resolve_framing] outer_pre:pre_t)
   (#[@resolve_framing] pre_f:pre_t)
-  (#[@resolve_framing] post_f:post_t a)
-  (#[@resolve_framing] post_g:post_t b)
   (#[@resolve_framing] frame_f:hprop)
   (#[@resolve_framing] _u:squash (can_be_split_into outer_pre pre_f frame_f))
-  (#[@resolve_framing] frame_g:hprop)
+
+  (#[@resolve_framing] post_f:post_t a)
   (#[@resolve_framing] pre_g:post_t a)
+  (#[@resolve_framing] frame_g:post_t a)
   (#[@resolve_framing] _v:squash (can_be_split_into_forall
     (fun x -> post_f x `star` frame_f) pre_g frame_g))
+
+  (#[@resolve_framing] post_g:a -> post_t b)
+  (#[@resolve_framing] outer_post:post_t b)
+  (#[@resolve_framing] _w:squash (can_be_split_into_forall_2 outer_post post_g frame_g))
+
   (f:repr a pre_f post_f)
-  (g:(x:a -> repr b (pre_g x) post_g))
-: repr b outer_pre (fun y -> post_g y `star` frame_g)
+  (g:(x:a -> repr b (pre_g x) (post_g x)))
+: repr b outer_pre outer_post
 = admit()
 
-let subcomp (a:Type) (pre:pre_t) (post:post_t a)
+let subcomp
+  (a:Type) (pre:pre_t) (post:post_t a)
   (f:repr a pre post)
 : Pure (repr a pre post)
   (requires True)
   (ensures fun _ -> True)
-= f
+= admit() //f
 
 
 let if_then_else (a:Type) (pre:pre_t) (post:post_t a)
@@ -99,16 +127,20 @@ inline_for_extraction noextract let resolve_frame () : Tac unit =
   canon()
 
 inline_for_extraction noextract let resolve_frame_forall () : Tac unit =
-  T.dump "entering resolve forall";
   ignore (forall_intro ());
-  T.dump "before resolve";
   resolve_frame()
+
+inline_for_extraction noextract let resolve_frame_forall_2 () : Tac unit =
+  ignore (forall_intro ());
+  ignore (forall_intro ());
+  resolve_frame()
+
 
 [@(resolve_implicits)
   (resolve_framing)]
 let resolve () : Tac unit =
     let rec aux (i:int) : Tac unit =
-//    T.dump ("State: " ^ string_of_int i);
+    T.dump ("State: " ^ string_of_int i);
     match T.goals () with
     | [] -> ()
     | g :: _ ->
@@ -139,18 +171,26 @@ let resolve () : Tac unit =
                   if T.term_eq hd (quote (can_be_split_into_forall)) then (
                     T.focus resolve_frame_forall;
                     aux (i+1)
-                  ) else T.fail "this is not an equality or a framing goal"
-                | _ -> T.fail "this is not an equality or a framing goal"
+                  ) else begin
+                    match T.inspect hd with
+                    | Tv_App hd _ ->
+                    if T.term_eq hd (quote (can_be_split_into_forall_2)) then (
+                      T.focus resolve_frame_forall_2;
+                      aux (i+1)
+                    ) else  T.fail "this is not an equality or a framing goal 1"
+                    | _ -> T.fail "this is not an equality or a framing goal 2"
+                  end
+                | _ -> T.fail "this is not an equality or a framing goal 3"
                 end
-            | _ -> T.fail "this is not an equality or a framing goal"
+            | _ -> T.fail "this is not an equality or a framing goal 4"
           end
-          | _ -> T.fail "this is not an equality or a framing goal"
+          | _ -> T.fail "this is not an equality or a framing goal 5"
           end
-        | _ -> T.fail "this is not an equality or a framing goal"
+        | _ -> T.fail "this is not an equality or a framing goal 6"
         end
 
       | _ -> // framing should have been handled beforehand
-        T.fail "this is not an equality or a framing goal"
+        T.fail "this is not an equality or a framing goal 7"
   in
   aux 0
 
@@ -167,10 +207,27 @@ val dependent_provides (_:unit)
 assume
 val nop (_:unit) : SteelT unit emp (fun c -> emp)
 
+assume
+val h_admit (#a:Type)
+             (#[@resolve_framing] p:hprop)
+             (#[@resolve_framing] q:a -> hprop)
+             (_:unit) : SteelT a p q
+
 //#push-options "--print_implicits --debug_level ResolveImplicitsHook"
+assume
+val ret (#a:Type) (x:a) (p:a -> hprop)
+  : SteelT a (p x) p
+
 val test_ok1 (_:unit)
   : SteelT myref emp (fun x -> myref_hprop x)
+
 let test_ok1 _
   = let tr = dependent_provides () in
-    nop ();
-    tr
+    // h_admit #_ #(myref_hprop tr) #myref_hprop ()
+    // AF: This does not work because of scoping issues on myref_hprop tr
+    nop();
+
+    ret tr myref_hprop
+
+    // nop ();
+    // tr
